arm/proofs/mlkem_basemul_k2.ml
@@ -400,14 +400,14 @@ let MLKEM_BASEMUL_K2_SUBROUTINE_CORRECT = prove
 needs "arm/proofs/consttime.ml";;
 needs "arm/proofs/subroutine_signatures.ml";;
 
-let full_spec = mk_safety_spec
+let full_spec,public_vars = mk_safety_spec
     (assoc "mlkem_basemul_k2" subroutine_signatures)
     MLKEM_BASEMUL_K2_SUBROUTINE_CORRECT
     MLKEM_BASEMUL_K2_EXEC;;
 
 let MLKEM_BASEMUL_K2_SUBROUTINE_SAFE = time prove
  (`exists f_events.
-       forall srcA srcB srcBt dst pc stackpointer returnaddress.
+       forall e srcA srcB srcBt dst pc stackpointer returnaddress.
            aligned 16 stackpointer /\
            ALLPAIRS nonoverlapping
            [dst,512; word_sub stackpointer (word 64),64]
@@ -418,8 +418,8 @@ let MLKEM_BASEMUL_K2_SUBROUTINE_SAFE = time prove
                (\s.
                     aligned_bytes_loaded s (word pc) mlkem_basemul_k2_mc /\
                     read PC s = word pc /\
-                    read X30 s = returnaddress /\
                     read SP s = stackpointer /\
+                    read X30 s = returnaddress /\
                     C_ARGUMENTS [dst; srcA; srcB; srcBt] s /\
                     read events s = e)
                (\s.
@@ -435,5 +435,5 @@ let MLKEM_BASEMUL_K2_SUBROUTINE_SAFE = time prove
                          word_sub stackpointer (word 64),64]
                         [dst,512; word_sub stackpointer (word 64),64])
                (\s s'. true)`,
-  ASSERT_GOAL_TAC full_spec THEN
-  PROVE_SAFETY_SPEC MLKEM_BASEMUL_K2_EXEC);;
+  ASSERT_CONCL_TAC full_spec THEN
+  PROVE_SAFETY_SPEC ~public_vars:public_vars MLKEM_BASEMUL_K2_EXEC);;
